

The cost function: 

$$
l(z, v) = \frac{1}{2}(z)^T Q_z (z) + \frac{1}{2}v^T R_v v
$$

The first derivatives with respect to:

* **$z$**:

$$
D_1 l = \frac{\partial l}{\partial z} =  Q_z * z \Rightarrow a_z(t)
$$

* **$v$**:

$$
D_2 l = \frac{\partial l}{\partial v} =  R_v * v \Rightarrow b_v(t)
$$

Quadratic approximation:

* $z(t)$: deviation in state
* $v(t)$: deviation in control

Therefore,

$$
a_z(t) =  Q z(t), \quad b_v(t) =  R v(t)
$$



##Construct Matrix $M$ and Vectors $m_1, m_2$


* From equation 7 we can find v(t):

$$
v(t) = -R_v^{-1} B(t)^T p(t)
$$

* Plugging this into equation 9:

$$
\dot{z}(t) = A(t)z(t) + B(t)v(t) \Rightarrow \dot{z}(t) = A(t)z(t) - B(t)R_v^{-1} B(t)^T p(t)
$$


* Plug a_z into equation 10:

$$
\dot{p}(t) = A(t)^T p(t) - Q_z z(t)
$$

Thus:



$$
M(t) = 
\begin{bmatrix}
A(t) & -B(t) R_v^{-1} B(t)^T \\
Q_z & A(t)^T
\end{bmatrix}, \quad m_1 = 0, \quad m_2 = 0
$$


Once z(t) and p(t) are solved then v(t) is found using the equation: 

$$
v(t) = -R_v^{-1} B(t)^T p(t)
$$


